causality: if expression evaluates, then it is causal up to some depth

src/Pipit.Exp.Causality.fst
@@ -28,16 +28,16 @@ let rec causal (e: exp): bool =
   | XPre e1 -> causal e1
   | XMu e1 -> causal e1 && not (direct_dependency e1 (XVar 0))
 
-// (* Causality: does expression `e` have a dependency on the most-recent value of variable `x`?
-//    Non-causal expressions cannot be evaluated with the bigstep semantics. *)
-// let rec direct_dependency (e: exp) (x: var) : bool =
-//   match e with
-//   | XVal _ -> false
-//   | XVar x' -> x = x'
-//   | XPrim2 _ e1 e2 -> direct_dependency e1 x || direct_dependency e2 x
-//   | XThen e1 e2 -> direct_dependency e1 x || direct_dependency e2 x
-//   | XPre _ -> false
-//   | XMu e1 -> direct_dependency e1 (x + 1)
+let rec causal_up_to_depth (e: exp) (n: nat): bool =
+  if n = 0 then true
+  else
+    match e with
+    | XVal _ -> true
+    | XVar x' -> true
+    | XPrim2 _ e1 e2 -> causal_up_to_depth e1 n && causal_up_to_depth e2 n
+    | XThen e1 e2 -> causal_up_to_depth e1 n && causal_up_to_depth e2 n
+    | XPre e1 -> causal_up_to_depth e1 (n - 1)
+    | XMu e1 -> causal_up_to_depth e1 n && not (direct_dependency e1 (XVar 0))
 
 let rec lift_inj (e e': exp) (x: var):
   Lemma (ensures (e = e') == (lift e x = lift e' x)) =
@@ -72,7 +72,7 @@ let rec direct_dependency_lift (e e': exp) (x: var):
     lift_lift_commute e' x 0;
     ()
 
-let rec direct_dependency_subst (x: var) (x': var { x' < x })
+let rec direct_dependency_not_subst (x: var) (x': var { x' < x })
   (e: exp { ~ (direct_dependency e (XVar x)) })
   (p: exp { ~ (direct_dependency p (XVar (x - 1))) }):
     Lemma (ensures ~ (direct_dependency (subst e x' p) (XVar (x - 1)))) (decreases e) =
@@ -80,15 +80,51 @@ let rec direct_dependency_subst (x: var) (x': var { x' < x })
   | XVal _ -> ()
   | XVar x'' -> ()
   | XPrim2 prim e1 e2 ->
-    direct_dependency_subst x x' e1 p;
-    direct_dependency_subst x x' e2 p
+    direct_dependency_not_subst x x' e1 p;
+    direct_dependency_not_subst x x' e2 p
   | XPre _ -> ()
   | XThen e1 e2 ->
-    direct_dependency_subst x x' e1 p;
-    direct_dependency_subst x x' e2 p
+    direct_dependency_not_subst x x' e1 p;
+    direct_dependency_not_subst x x' e2 p
   | XMu e1 ->
     direct_dependency_lift p (XVar (x - 1)) 0;
-    direct_dependency_subst (x + 1) (x' + 1) e1 (lift p 0)
+    direct_dependency_not_subst (x + 1) (x' + 1) e1 (lift p 0)
+
+let rec direct_dependency_not_subst2 (x: var) (x': var { x < x' }) (e p: exp):
+    Lemma
+      (requires not (direct_dependency (subst e x' p) (XVar x)))
+      (ensures not (direct_dependency e (XVar x))) (decreases e) =
+  match e with
+  | XVal _ -> ()
+  | XVar x'' -> ()
+  | XPrim2 prim e1 e2 ->
+    direct_dependency_not_subst2 x x' e1 p;
+    direct_dependency_not_subst2 x x' e2 p
+  | XPre _ -> ()
+  | XThen e1 e2 ->
+    direct_dependency_not_subst2 x x' e1 p;
+    direct_dependency_not_subst2 x x' e2 p
+  | XMu e1 ->
+    direct_dependency_lift p (XVar x') 0;
+    direct_dependency_not_subst2 (x + 1) (x' + 1) e1 (lift p 0)
+
+let rec causal_up_to_depth_lift (e: exp) (x: var) (n: nat):
+    Lemma (ensures causal_up_to_depth e n == causal_up_to_depth (lift e x) n) =
+  match e with
+  | XVal _ -> ()
+  | XVar _ -> ()
+  | XPrim2 p e1 e2 ->
+    causal_up_to_depth_lift e1 x n;
+    causal_up_to_depth_lift e2 x n
+  | XPre e1 -> if n > 0 then causal_up_to_depth_lift e1 x (n - 1)
+  | XThen e1 e2 ->
+    causal_up_to_depth_lift e1 x n;
+    causal_up_to_depth_lift e2 x n
+  | XMu e1 ->
+    causal_up_to_depth_lift e1 (x + 1) n;
+    lift_lift_commute e1 (x + 1) 0;
+    direct_dependency_lift e1 (XVar 0) (x + 1)
+
 
 let rec bigstep_no_dep_no_difference (#outer #inner1 #inner2: nat) (e: exp { ~ (direct_dependency e (XVar inner1)) })
   (streams1: C.table (outer + 1) inner1)
@@ -142,18 +178,127 @@ let rec bigstep_no_dep_no_difference (#outer #inner1 #inner2: nat) (e: exp { ~ (
     BSThen _ e1 e2 vs1 vs2 hBS1' hBS2'
   | BSMu _ e1 vs1 hBS1 ->
     let e1' = subst e1 0 (XMu e1) in
-    direct_dependency_subst (inner1 + 1) 0 e1 (XMu e1);
+    direct_dependency_not_subst (inner1 + 1) 0 e1 (XMu e1);
     let hBS1' = bigstep_no_dep_no_difference e1' streams1 streams2 row v v' vs1 hBS1 in
     BSMu _ e1 vs1 hBS1'
 
 
-let bigstep_recursive_XMu (#outer #inner: nat) (e: exp { causal (XMu e) })
+(* I originally thought that something like the following should hold:
+   if e evaluates to a value, then e is causal
+   but this doesn't work for empty input streams, and also doesn't work for
+   recursive binders that are nested arbitrarily inside pre combinators, eg
+   > pre (pre (pre (pre (mu x. x))))
+
+*)
+// let rec bigstep_means_causal (#outer #inner: nat) (e: exp)
+//   (streams: C.table outer inner)
+//   (vs: C.vector value outer)
+//   (hBS: bigstep streams e vs):
+//     Lemma (ensures causal e) (decreases hBS) =
+//
+
+let rec causal_up_to_subst1 (e e': exp) (x: var) (n: nat):
+  Lemma (requires causal_up_to_depth (subst e x e') n)
+        (ensures causal_up_to_depth e n) =
+  if n = 0 then ()
+  else
+    match e with
+    | XPrim2 _ e1 e2 -> causal_up_to_subst1 e1 e' x n; causal_up_to_subst1 e2 e' x n
+    | XMu e1 ->
+      causal_up_to_subst1 e1 (lift e' 0) (x + 1) n;
+      direct_dependency_not_subst2 0 (x + 1) e1 (lift e' 0);
+      ()
+    | XPre e1 -> causal_up_to_subst1 e1 e' x (n - 1)
+    | XThen e1 e2 -> causal_up_to_subst1 e1 e' x n; causal_up_to_subst1 e2 e' x n
+    | _ -> ()
+
+let rec direct_dep_XVar__direct_dep_subst (e e': exp) (x: var):
+  Lemma (requires direct_dependency e (XVar x))
+        (ensures direct_dependency (subst e x e') e') =
+  match e with
+  | XPrim2 _ e1 e2 ->
+    if direct_dependency e1 (XVar x)
+    then direct_dep_XVar__direct_dep_subst e1 e' x
+    else direct_dep_XVar__direct_dep_subst e2 e' x
+  | XMu e1 ->
+    direct_dep_XVar__direct_dep_subst e1 (lift e' 0) (x + 1)
+  | XThen e1 e2 ->
+    if direct_dependency e1 (XVar x)
+    then direct_dep_XVar__direct_dep_subst e1 e' x
+    else direct_dep_XVar__direct_dep_subst e2 e' x
+  | _ -> ()
+
+let rec direct_dep_acausal__acausal (e e': exp) (n: nat):
+  Lemma (requires direct_dependency e e' /\ not (causal_up_to_depth e' n))
+        (ensures not (causal_up_to_depth e n)) =
+  if e = e' then ()
+  else
+  match e with
+  | XPrim2 p e1 e2 ->
+    if direct_dependency e1 e'
+    then direct_dep_acausal__acausal e1 e' n
+    else direct_dep_acausal__acausal e2 e' n
+  | XMu e1 ->
+    assert (direct_dependency e1 (lift e' 0));
+    causal_up_to_depth_lift e' 0 n;
+    direct_dep_acausal__acausal e1 (lift e' 0) n;
+    ()
+  | XThen e1 e2 ->
+    if direct_dependency e1 e'
+    then direct_dep_acausal__acausal e1 e' n
+    else direct_dep_acausal__acausal e2 e' n
+  | _ -> ()
+
+let causal_up_to_depth_subst_XMu (e: exp) (n: nat):
+  Lemma (requires causal_up_to_depth (subst e 0 (XMu e)) n)
+        (ensures causal_up_to_depth (XMu e) n) =
+  if n = 0
+  then ()
+  else begin
+    if direct_dependency e (XVar 0)
+    then
+    begin
+      assert (not (causal_up_to_depth (XMu e) n));
+      direct_dep_XVar__direct_dep_subst e (XMu e) 0;
+      direct_dep_acausal__acausal (subst e 0 (XMu e)) (XMu e) n;
+      ()
+    end
+    else
+      causal_up_to_subst1 e (XMu e) 0 n
+  end
+
+
+let rec bigstep_means_causal_up_to_depth (#outer #inner: nat) (e: exp)
+  (streams: C.table outer inner)
+  (vs: C.vector value outer)
+  (hBS: bigstep streams e vs):
+    Lemma (ensures causal_up_to_depth e outer) (decreases hBS) =
+  match hBS with
+  | BSVal _ _ -> ()
+  | BSVar _ x' -> ()
+  | BSPrim2 _ p e1' e2' vs1 vs2 hBS1 hBS2 ->
+    let XPrim2 _ e1 e2 = e in
+    bigstep_means_causal_up_to_depth e1 streams vs1 hBS1;
+    bigstep_means_causal_up_to_depth e2 streams vs2 hBS2
+  | BSMu _ e1' vs1 hBS1 ->
+    let XMu e1 = e in
+    bigstep_means_causal_up_to_depth (subst e1 0 (XMu e1)) streams vs1 hBS1;
+    causal_up_to_depth_subst_XMu e1 outer
+  | BSPre _ streams' e1 vs1 hBS1 ->
+    bigstep_means_causal_up_to_depth e1 streams' vs1 hBS1
+  | BSPre0 _ -> ()
+  | BSThen _ e1 e2 vs1 vs2 hBS1 hBS2 ->
+    bigstep_means_causal_up_to_depth e1 streams vs1 hBS1;
+    bigstep_means_causal_up_to_depth e2 streams vs2 hBS2
+
+
+let bigstep_recursive_XMu (#outer #inner: nat) (e: exp)
   (streams: C.table (outer + 1) inner)
   (vs: C.vector value outer) (v v': value)
   (hBSmu: bigstep streams (XMu e) (v :: vs)):
     bigstep (C.table_map_append (C.table_of_values (v' :: vs)) streams) e (v :: vs) =
+    bigstep_means_causal_up_to_depth _ _ _ hBSmu;
     let hBS' = bigstep_substitute_XMu e streams _ hBSmu in
     C.table_map_append_empty1 (C.table_map_append (C.table_of_values (v :: vs)) streams);
     C.table_map_append_empty1 (C.table_map_append (C.table_of_values (v' :: vs)) streams);
     bigstep_no_dep_no_difference e (C.table_empty (outer + 1)) streams vs v v' (v :: vs) hBS'
-
